add: per-jit shift proof

theory/JITFlat.thy
@@ -1,7 +1,192 @@
 theory JITFlat
 
-imports JITPer_aux
+imports JITPer_aux JITPer
 begin
+
+
+type_synonym flat_bpf_prog = "x64_bin \<times> (u64 \<times> nat) list \<times> ((u64\<times>u64) list)"
+
+(*fun jitflat_bpf :: "(nat \<times> u64 \<times> x64_bin) list \<Rightarrow> flat_bpf_prog \<Rightarrow> flat_bpf_prog" where
+"jitflat_bpf [] st = st"| 
+"jitflat_bpf ((num,off,l_bin0)#xs) (l_bin,l_pc,l_jump) = (
+  let curr_pc = of_nat (length l_bin) in 
+    if l_bin0!0 = (0x0f::u8) then \<comment>\<open> TODO: if the first byte is the opcode of cmp? \<close>
+      jitflat_bpf xs (
+        l_bin@l_bin0,
+        l_pc@[(curr_pc,num)],
+        l_jump@ [(of_nat (length l_pc), of_nat (length l_pc) + off)])
+    else
+      jitflat_bpf xs (l_bin@l_bin0, l_pc@[(curr_pc,num)], l_jump)
+)"*)
+
+
+fun jitflat_bpf :: "(nat \<times> u64 \<times> x64_bin) list \<Rightarrow> flat_bpf_prog \<Rightarrow> flat_bpf_prog" where
+"jitflat_bpf [] st = st"| 
+"jitflat_bpf ((num,off,l_bin0)#xs) (l_bin,l_pc,l_jump) = (
+      jitflat_bpf xs (l_bin@l_bin0, l_pc@[(of_nat (length l_bin),num)],if l_bin0!0 = (0x0f::u8) then l_jump@ [(of_nat (length l_pc), of_nat (length l_pc) + off)]
+                   else l_jump)
+)"
+
+fun find_target_pc_in_l_pc :: "((u64\<times>u64) list) \<Rightarrow> u64 \<Rightarrow> u64 option" where
+"find_target_pc_in_l_pc [] _ = None" |
+"find_target_pc_in_l_pc ((x, y)#xs) pc = (
+  if x = pc then Some y
+  else find_target_pc_in_l_pc xs pc
+)"
+
+definition init_second_layer::"x64_bin \<times> (u64 \<times> nat) list \<times> ((u64\<times>u64) list)" where
+"init_second_layer \<equiv> ([],[],[])"
+
+
+definition flat_bpf_one_step :: "u64 \<Rightarrow> nat \<Rightarrow> flat_bpf_prog \<Rightarrow> hybrid_state \<Rightarrow> hybrid_state" where
+"flat_bpf_one_step xpc num lp st = (
+
+  let (l_bin,l_pc,l_jump) = lp in
+  let (pc, xst) = st in
+    case xst of
+    Stuck \<Rightarrow> (pc, Stuck) |
+    Next xpc_old rs m \<Rightarrow> (
+      if xpc \<noteq> xpc_old then \<comment>\<open> In this case, xpc should be equal to xpc_old \<close>
+        (pc, Stuck)
+      else
+        if l_bin!(unat xpc+1) = (0x39::u8) then \<comment>\<open> TODO: if the first byte is the opcode of cmp? \<close>
+          \<comment>\<open> case: BPF JMP \<close>
+          case x64_sem 1 l_bin (Next xpc rs m) of
+          Stuck \<Rightarrow> (pc, Stuck) | \<comment>\<open> if one step error, stop, it should be impossible \<close>
+          Next xpc1 rs1 m1 \<Rightarrow> (
+            if rs1 (CR ZF) = 1 then \<comment>\<open> must JUMP \<close>
+              case find_target_pc_in_l_pc l_jump pc of
+              None \<Rightarrow> (pc, Stuck) |
+              Some npc \<Rightarrow>
+                (npc, (Next (fst (l_pc!(unat npc))) rs1 m1)) \<comment>\<open> go to the target address in the jited x64 binary \<close>
+            else \<comment>\<open> donot JUMP \<close>
+              (pc+1, xst)
+          )
+         else
+          \<comment>\<open> case: NOT BPF JMP \<close>
+          (pc+1, x64_sem num l_bin (Next xpc rs m))
+))"
+
+fun flat_bpf_sem :: "nat \<Rightarrow> flat_bpf_prog \<Rightarrow> hybrid_state \<Rightarrow> hybrid_state" where
+"flat_bpf_sem 0 _ hst = hst" |
+"flat_bpf_sem (Suc n) (l_bin,l_pc,l_jump) (pc, xst) = (
+  let (xpc, num) = l_pc!(unat pc) ;
+   (npc, nxst) = flat_bpf_one_step xpc num (l_bin,l_pc,l_jump) (pc, xst) in
+  flat_bpf_sem n (l_bin,l_pc,l_jump) (npc, nxst)
+)"
+
+value "jitflat_bpf [(1, 1, [0x48,0x01,0xD8]),(1, 2, [0x0f, 0x84, 0x00, 0x00, 0x00, 0x00]), (1, 1, [0x48,0x01,0xD8]), (1, 1, [0x48,0x01,0xD8])] init_second_layer"
+
+value "jitflat_bpf [(1, 2, [0x0f, 0x84, 0x00, 0x00, 0x00, 0x00]), (1, 1, [0xc3]), (1, 1, [0x48,0x01,0xD8]), (1, 1, [0x48,0x01,0xD8]),(1, -3, [0x0f, 0x84, 0x00, 0x00, 0x00, 0x00])] init_second_layer"
+
+
+lemma 
+  "l_bin!pc=(num,off,l) \<Longrightarrow>
+  jitflat_bpf l_bin (l1,l_pc1,l_jump1) = (l2,l_pc2,l_jump2) \<Longrightarrow>
+  fst (l_pc2 ! (length l_pc1 + pc) ) = xpc \<Longrightarrow>
+  list_in_list l (length l1 + unat xpc) l2"
+
+lemma one_step_equiv:
+ (* "flat_bpf_one_step xpc num (l_bin,l_pc,l_jump) (pc, xst) = fxst \<Longrightarrow>
+   jitflat_bpf lt init_second_layer = (l_bin,l_pc,l_jump) \<Longrightarrow>
+   one_step lt (pc,xst) = xxst \<Longrightarrow>
+   fxst = xxst"*)
+  assumes a0:"flat_bpf_one_step xpc num (l_bin,l_pc,l_jump) (pc, xst) = fxst" and
+   a1:"jitflat_bpf lt init_second_layer = (l_bin,l_pc,l_jump)" and
+   a2:"one_step lt (pc,xst) = xxst" and
+   a3:"xst = Next xpc xrs xm"
+  shows"fxst = xxst"
+ (*proof-
+  have "l_pc!(unat pc) = "
+let "?l_bin0" = "map snd (map snd lt)"
+  have a4:"l_bin = concat ?l_bin0" using a1 jitflat_bpf.simps init_second_layer_def
+  have "l_bin!(unat xpc) = (0x0f::u8) \<or> l_bin!(unat xpc) \<noteq> (0x0f::u8)" by auto
+  thus ?thesis
+  proof(cases "l_bin!(unat xpc)  = (0x0f::u8)")
+    case True
+    then show ?thesis sorry
+  next
+    case False
+    have b0:"l_bin!(unat xpc) \<noteq> (0x0f::u8)" using False by simp
+    have b1:""
+    then show ?thesis sorry
+  qed*)
+  sorry
+
+
+
+lemma flat_bpf_sem_induct_aux1:
+ "flat_bpf_sem (m+n) x64_prog xst = xst'\<Longrightarrow> 
+  \<exists> xst1. flat_bpf_sem m x64_prog xst = xst1 \<and>
+  flat_bpf_sem n x64_prog xst1 = xst'"
+ apply(induct m arbitrary: n x64_prog xst xst' )
+   apply auto[1]
+  subgoal for m n x64_prog xst xst'
+    apply (simp add: Let_def)
+    apply(cases xst;simp)
+    subgoal for a b sorry
+    done
+  done
+
+lemma flat_bpf_sem_induct_aux2:
+"flat_bpf_sem (Suc n) x64_prog xst = xst'\<Longrightarrow> 
+  \<exists> xst1. flat_bpf_sem 1 x64_prog xst = xst1 \<and>
+  flat_bpf_sem n x64_prog xst1 = xst'"
+  using flat_bpf_sem_induct_aux1 by simp
+
+
+
+lemma one_step_equiv:
+ (* "flat_bpf_one_step xpc num (l_bin,l_pc,l_jump) (pc, xst) = fxst \<Longrightarrow>
+   jitflat_bpf lt init_second_layer = (l_bin,l_pc,l_jump) \<Longrightarrow>
+   one_step lt (pc,xst) = xxst \<Longrightarrow>
+   fxst = xxst"*)
+  assumes a0:"flat_bpf_one_step xpc num (l_bin,l_pc,l_jump) (pc, xst) = fxst" and
+   a1:"jitflat_bpf lt init_second_layer = (l_bin,l_pc,l_jump)" and
+   a2:"one_step lt (pc,xst) = xxst" and
+   a3:"xst = Next xpc xrs xm"
+ shows"fxst = xxst"
+  sorry
+
+
+
+lemma n_steps_equiv:
+  "flat_bpf_sem n prog xst = fxst \<Longrightarrow>
+  jitflat_bpf lt init_second_layer = prog \<Longrightarrow>
+  x64_sem1 n lt xst = xxst \<Longrightarrow>
+  snd xst = Next xpc xrs xm \<Longrightarrow>
+  fxst = xxst"
+proof(induct n)
+  case 0
+  then show ?case 
+    by (metis flat_bpf_sem.simps(1) prod.collapse x64_sem1.simps(1))
+next
+  case (Suc n)
+  assume assm0:"flat_bpf_sem (Suc n) prog xst = fxst" and 
+  assm1:"jitflat_bpf lt init_second_layer = prog" and
+  assm2:"x64_sem1 (Suc n) lt xst = xxst" and
+  assm3:"snd xst = Next xpc xrs xm"
+  have "\<exists> next_s. next_s = one_step lt xst" by simp
+  then obtain next_s where b0:"next_s = one_step lt xst" by auto
+  have "\<exists> next_f num. flat_bpf_one_step xpc num prog xst = next_f" by blast
+  then obtain next_f num where b1:"flat_bpf_one_step xpc num prog xst = next_f" by simp
+  have bn:"next_s = next_f" using  assm1 b0 b1 assm3 one_step_equiv 
+    by (metis prod.collapse)
+  have "\<exists> xrs1 xpc1 m1. snd next_s = Next xrs1 xpc1 m1" sorry
+  then obtain xrs1 xpc1 m1 where b2:"snd next_s = Next xrs1 xpc1 m1" by auto
+
+  have "flat_bpf_sem n prog xst = fxst" using flat_bpf_sem_induct_aux2 assm0 b1 sorry
+  
+  have "flat_bpf_sem n prog xst = fxst \<Longrightarrow>
+    jitflat_bpf lt init_second_layer = prog \<Longrightarrow> 
+    x64_sem1 n lt xst = xxst \<Longrightarrow> 
+    snd xst = Next xpc xrs xm \<Longrightarrow> 
+    fxst = xxst" using Suc by blast
+  have "fxst = xxst" using x64_sem1_induct_aux3 flat_bpf_sem_induct_aux1 bn Suc b2 
+  then show ?case sorry
+qed
+
+(*
 
 type_synonym l_pc = "u64 list"
 
@@ -141,9 +326,6 @@ fun jitfix :: "l_jump \<Rightarrow> x64_bin \<Rightarrow> l_pc \<Rightarrow> x64
                               l' = x64_bin_update l (unat (fix_begin_addr+2)) u8_list in 
                           jitfix xs l' pcs)"
 
-value "jitflat [(1, 1, [0x48,0x01,0xD8]),(1, 2, [0x0f, 0x84, 0x00, 0x00, 0x00, 0x00]), (1, 1, [0x48,0x01,0xD8]), (1, 1, [0x48,0x01,0xD8])] init_second_layer"
-
-value "jitflat [(1, 2, [0x0f, 0x84, 0x00, 0x00, 0x00, 0x00]), (1, 1, [0xc3]), (1, 1, [0x48,0x01,0xD8]), (1, 1, [0x48,0x01,0xD8]),(1, -3, [0x0f, 0x84, 0x00, 0x00, 0x00, 0x00])] init_second_layer"
 
 value "jitfix [(1::64 word, 3::64 word)] 
   [72::8 word, 1::8 word, 216::8 word, 15::8 word, 132::8 word, 0::8 word, 0::8 word, 0::8 word, 0::8 word, 72::8 word, 1::8 word, 216::8 word, 72::8 word, 1::8 word, 216::8 word] 
@@ -258,6 +440,6 @@ definition jitflat3 :: "(nat \<times> u64 \<times> x64_bin) list \<Rightarrow> (
 
 
                               
-
+*)
 
 end
